Bdd/Unused.lean
@@ -1,0 +1,253 @@
+module
+
+import all Bdd.Basic
+import all Bdd.Size
+
+section not_used
+open Pointer
+
+inductive Pointer.le {m} : Pointer m → Pointer m → Prop where
+  | terminal_le_terminal {b c} : b ≤ c → le (terminal b) (terminal c)
+  | terminal_le_node {b j} : le (terminal b) (node j)
+  | node_le_node {j i} : j ≤ i → le (node j) (node i)
+
+instance Pointer.instLE : LE (Pointer m) := {le := Pointer.le}
+
+instance Pointer.instDecidableLe {m} : DecidableLE (Pointer m) :=
+  fun p q ↦ match p with
+  | terminal b => match q with
+    | terminal c => match Bool.instDecidableLe b c with
+      | isTrue ht => isTrue  (.terminal_le_terminal ht)
+      | isFalse hf => isFalse (by intro contra; cases contra; contradiction)
+    | node i => isTrue (.terminal_le_node)
+  | node j => match q with
+    | terminal c => isFalse (by intro contra; contradiction)
+    | node i => match Fin.decLe j i with
+      | isTrue ht => isTrue (.node_le_node ht)
+      | isFalse hf => isFalse (by intro contra; cases contra; contradiction)
+
+@[simp]
+def Pointer.MayPrecede {n m} (M : Vector (Node n m) m) (p q : Pointer m) := toVar M p < toVar M q
+
+/-- Terminals must not precede other pointers. -/
+@[simp, grind .]
+lemma Pointer.not_terminal_mayPrecede : ¬ MayPrecede M (terminal b) p := by
+  cases p with
+  | terminal _ => simp [MayPrecede]
+  | node     j => exact not_lt.mpr (Fin.le_last _)
+
+/-- Non-terminals may precede terminals. -/
+lemma Pointer.MayPrecede_node_terminal {n m} (w : Vector (Node n m) m) {j b} : MayPrecede w (node j) (terminal b) := by
+  simp only [MayPrecede, Nat.succ_eq_add_one, toVar, Fin.getElem_fin]
+  refine Fin.mk_lt_of_lt_val ?_
+  simp only [Fin.val_last, Fin.is_lt]
+
+def OBdd.OReachable {n m} := Relation.ReflTransGen (@OEdge n m)
+
+lemma OBdd.low_oreachable {n m} {j} {O U : OBdd n m} {U_root_def : U.1.root = node j}:
+    O.OReachable U → O.OReachable (U.low U_root_def) :=
+  fun h ↦ Relation.ReflTransGen.tail h oedge_of_low
+
+lemma OBdd.high_oreachable {n m} {j} {O U : OBdd n m} {U_root_def : U.1.root = node j} :
+    O.OReachable U → O.OReachable (U.high U_root_def) :=
+  fun h ↦ Relation.ReflTransGen.tail h oedge_of_high
+
+lemma aux {O : OBdd n m} {i : Fin m} :
+    O.1.heap[i.1].var = Fin.castPred (toVar O.1.heap (node i)) (Fin.exists_castSucc_eq.mp ⟨O.1.heap[i.1].var, by simp [toVar]; rfl⟩) :=
+  by simp [toVar]
+
+/-- The output of equal constant functions with inhabited domain is equal. -/
+lemma eq_of_constant_eq {α β} {c c' : β} [Inhabited α] :
+    Function.const α c = Function.const α c' → c = c' :=
+  fun h ↦ (show (Function.const α c) default = (Function.const α c') default by rw [h])
+
+lemma OBdd.reachable_node_iff {n m j} {O : OBdd n m} (h : O.1.root = node j) :
+  Reachable O.1.heap O.1.root = fun q ↦
+    (Reachable O.1.heap O.1.root q ∧ ¬ Reachable O.1.heap (O.low h).1.root q ∧ ¬ Reachable O.1.heap (O.high h).1.root q) ∨
+    (Reachable O.1.heap (O.low  h).1.root q ∧ ¬ Reachable O.1.heap (O.high h).1.root q) ∨
+    (Reachable O.1.heap (O.high h).1.root q ∧ ¬ Reachable O.1.heap (O.low  h).1.root q) ∨
+    (Reachable O.1.heap (O.low  h).1.root q ∧   Reachable O.1.heap (O.high h).1.root q) := by
+  ext p
+  constructor
+  · intro r
+    cases instDecidableReachable (O.low h) p with
+    | isFalse hf =>
+      cases instDecidableReachable (O.high h) p with
+      | isFalse hhf =>
+        left
+        exact ⟨r, hf, hhf⟩
+      | isTrue hht =>
+        right
+        right
+        left
+        exact ⟨hht, hf⟩
+    | isTrue ht =>
+      cases instDecidableReachable (O.high h) p with
+      | isFalse hhf =>
+        right
+        left
+        exact ⟨ht, hhf⟩
+      | isTrue hht =>
+        right
+        right
+        right
+        exact ⟨ht, hht⟩
+  · intro r
+    cases r with
+    | inl r => exact r.1
+    | inr r =>
+      cases r with
+      | inl r =>
+        trans (O.low h).1.root
+        · exact O.bdd.reachable_low h
+        · exact r.1
+      | inr r =>
+        cases r with
+        | inl r =>
+          trans (O.high h).1.root
+          · exact O.bdd.reachable_high h
+          · exact r.1
+        | inr r =>
+          trans (O.high h).1.root
+          · exact O.bdd.reachable_high h
+          · exact r.2
+
+/-- Similarity of `Ordered` BDDs is decidable. -/
+instance OBdd.instDecidableSimilar {n m} : DecidableRel (β := OBdd n m) OBdd.Similar :=
+  fun O U ↦ decidable_of_decidable_of_iff (show O.toTree = U.toTree ↔ _ by simp [Similar, HSimilar])
+
+-- FIXME: Use the instance from Sim.lean instead.
+instance OBdd.instDecidableHSimilar {n m m'} (O : OBdd n m) (U : OBdd n m') : Decidable (OBdd.HSimilar O U) :=
+  decidable_of_decidable_of_iff (show O.toTree = U.toTree ↔ _ by simp [HSimilar])
+
+@[no_expose]
+instance OBdd.instDecidableSimilarRP : Decidable (OBdd.SimilarRP O l r) := by
+  simp only [OBdd.SimilarRP]; infer_instance
+
+instance OBdd.instFintypeRelevantPointer {n m} (O : OBdd n m) : Fintype (O.1.RelevantPointer) := by
+  convert Subtype.fintype _ <;> infer_instance
+
+@[implicit_reducible]
+def Pointer.decidableEitherReachable {n m} (O U : OBdd n m) (h : O.1.heap = U.1.heap) :
+    DecidablePred (fun q ↦ (Reachable O.1.heap O.1.root q) ∨ (Reachable O.1.heap U.1.root q)) := by
+  intro p
+  simp
+  cases instDecidableReachable O p with
+  | isFalse hf =>
+    cases instDecidableReachable U p with
+    | isFalse hhf =>
+      apply isFalse
+      simp_all [or_self, not_false_eq_true]
+    | isTrue  hht =>
+      apply isTrue
+      simp_all only [or_true]
+  | isTrue  ht =>
+    apply isTrue
+    simp_all only [true_or]
+
+@[implicit_reducible]
+def OBdd.fintypeEitherRelevantPointer (O U : OBdd n m) (h : O.1.heap = U.1.heap) :
+    Fintype { q // Reachable O.1.heap O.1.root q ∨ Reachable O.1.heap U.1.root q } := by
+  convert Subtype.fintype _
+  · exact decidableEitherReachable O U h
+  · infer_instance
+
+@[no_expose]
+instance OBdd.instFintypeReachableFromNode (O : OBdd n m) (h : O.1.root = node j) :
+    Fintype { q // q = O.1.root ∨ (Reachable O.1.heap (O.low  h).1.root q ∨ Reachable O.1.heap (O.high h).1.root q) } := by
+  convert Subtype.fintype _
+  · intro p
+    simp only
+    cases decEq p O.1.root with
+    | isFalse hf =>
+      cases instDecidableReachable (O.low h) p with
+      | isFalse hhf =>
+        cases instDecidableReachable (O.high h) p with
+        | isFalse hhhf =>
+          apply isFalse
+          simp
+          exact ⟨hf, hhf, hhhf⟩
+        | isTrue hhht =>
+          apply isTrue
+          right
+          right
+          assumption
+      | isTrue hht =>
+        apply isTrue
+        right
+        left
+        assumption
+    | isTrue h =>
+      apply isTrue
+      left
+      assumption
+  · infer_instance
+
+/-- The inverse image of a decidable relation is decidable. -/
+instance my_decidableRel_of_invImage2 {r : β → β → Prop} [DecidableRel r] {f : α → β} :
+    DecidableRel (InvImage r f) :=
+  fun a b ↦ decidable_of_decidable_of_iff (show (r (f a) (f b)) ↔ _ by simp [InvImage])
+
+instance Bdd.instDecidableEqRelevantPointer : DecidableEq (Bdd.RelevantPointer B) :=
+  fun _ _ ↦ decidable_of_iff _ (symm Subtype.ext_iff)
+
+/-- `Reduced` is decidable. -/
+@[no_expose]
+instance OBdd.instReducedDecidable {n m} : DecidablePred (α := OBdd n m) Reduced :=
+  fun _ ↦ (instDecidableAnd (dp := Fintype.decidableForallFintype) (dq := Fintype.decidableForallFintype))
+
+lemma OBdd.card_reachable_node' {O : OBdd n m} (h : O.1.root = node j) :
+  Fintype.card {p // Reachable O.1.heap O.1.root p} =
+  Fintype.card {p // p = O.1.root ∨ (Reachable O.1.heap (O.low  h).1.root p ∨ Reachable O.1.heap (O.high h).1.root p)} := by
+  apply Fintype.card_congr'
+  conv =>
+    lhs
+    arg 1
+    ext
+    rw [reachable_from_node_iff' h]
+
+lemma OBdd.card_reachable_node {n m j} {O : OBdd n m} (h : O.1.root = node j) :
+  Fintype.card { q // Reachable O.1.heap O.1.root q } =
+  1 + Fintype.card { q // Reachable (O.low h).1.heap (O.low h).1.root q ∨ Reachable (O.high h).1.heap (O.high h).1.root q } := by
+  rw [card_reachable_node' h]
+  rw [@Fintype.card_subtype_or_disjoint _ _ _ (eq_root_disjoint_reachable_low_or_high h) ..]
+  · simp only [Fintype.card_unique, low_heap_eq_heap, add_right_inj]
+    apply @Fintype.card_congr' ..
+    · apply fintypeEitherRelevantPointer (O.low h) (O.high h); simp
+    · simp
+  · exact Fintype.subtypeEq O.1.root
+
+@[no_expose, implicit_reducible]
+instance OBdd.instDecidableReachable' {n m} (O : OBdd n m) (p : O.1.RelevantPointer) q :
+    Decidable (Reachable O.1.heap p.val q) := by
+  rcases p with ⟨p, hp⟩
+  match p with
+  | terminal b =>
+    exact decidable_of_iff _ Reachable.terminal_iff.symm
+  | node j =>
+    let high := O.1.heap[j].high
+    let low := O.1.heap[j].low
+    suffices Decidable (q = node j ∨ Reachable O.bdd.heap high q ∨ Reachable O.bdd.heap low q) from
+      decidable_of_iff _ Bdd.reachable_node_iff.symm
+    refine @instDecidableOr _ _ ?_ (@instDecidableOr _ _ ?_ ?_)
+    · exact decEq ..
+    · have hr : Reachable O.1.heap O.1.root high :=
+        Reachable.snoc hp Edge.high
+      exact OBdd.instDecidableReachable' O ⟨high, hr⟩ q
+    · have hr : Reachable O.1.heap O.1.root low :=
+        Reachable.snoc hp Edge.low
+      exact OBdd.instDecidableReachable' O ⟨low, hr⟩ q
+termination_by p
+decreasing_by
+  all_goals simp_all only [flip, Bdd.RelevantEdge]
+  · exact Edge.high
+  · exact Edge.low
+
+namespace Size
+
+def bool_of_size_eq_zero {n m} (O : OBdd n m) (h : size O = 0) : Bool :=
+  match O_root_def : O.1.root with
+  | .terminal b => b
+  | .node _ => False.elim (not_isTerminal_of_root_eq_node O_root_def (isTerminal_iff_size_eq_zero.mp h))
+
+end Size
